theories/URI.v
@@ -1,0 +1,53 @@
+From Coq Require Export
+     DecidableClass.
+From HTTP Require Export
+     Common
+     Message.
+
+Program Instance Decidable_eq_scheme (x y : http_scheme) : Decidable (x = y) :=
+  { Decidable_witness :=
+      match x, y with
+      | Scheme__HTTP , Scheme__HTTP
+      | Scheme__HTTPS, Scheme__HTTPS => true
+      | Scheme s1  , Scheme s2 => s1 = s2?
+      | _, _ => false
+      end }.
+Solve Obligations with split; intuition; discriminate.
+Next Obligation.
+  destruct x, y; intuition; try discriminate; f_equal; apply eqb_eq; intuition.
+  inversion H; reflexivity.
+Qed.
+
+Program Instance Decidable_eq_authority (x y : authority) : Decidable (x = y) :=
+  { Decidable_witness :=
+      let 'Authority u1 h1 p1 := x in
+      let 'Authority u2 h2 p2 := y in
+      (u1 = u2?) &&& (h1 =? h2) &&& (p1 = p2?) }.
+Next Obligation.
+  intuition.
+  - destruct x, y.
+    do 2 (apply andb_true_iff in H; destruct H).
+    f_equal; apply Decidable_spec; intuition.
+  - subst.
+    destruct y.
+    destruct authority__userinfo, authority__port;
+      repeat (apply andb_true_iff; intuition);
+        try apply eqb_eq; try apply N.eqb_eq; reflexivity.
+Qed.
+
+Program Instance Decidable_eq_uri (x y : absolute_uri) : Decidable (x = y) :=
+  { Decidable_witness :=
+      let 'URI s1 a1 p1 oq1 := x in
+      let 'URI s2 a2 p2 oq2 := y in
+      (s1 = s2)? &&& (a1 = a2?) &&& (p1 =? p2) &&& (oq1 = oq2?) }.
+Next Obligation.
+  intuition.
+  - destruct x, y.
+    do 3 (apply andb_true_iff in H; destruct H).
+    f_equal; apply Decidable_spec; intuition.
+  - subst.
+    destruct y.
+    destruct uri__scheme, uri__authority, uri__query, authority__userinfo, authority__port;
+      repeat (apply andb_true_iff; intuition);
+      try apply eqb_eq; try apply N.eqb_eq; reflexivity.
+Qed.
